feat: more helper theorems

src/Init/Data/Int/Linear.lean
@@ -1915,6 +1915,11 @@ theorem eq_def (ctx : Context) (x : Var) (xPoly : Poly) (p : Poly)
   simp [eq_def_cert]; intro _ h; subst p; simp [h]
   rw [← Int.sub_eq_add_neg, Int.sub_self]
 
+theorem eq_def_norm (ctx : Context) (x : Var) (xPoly xPoly' : Poly) (p : Poly)
+    : eq_def_cert x xPoly' p → x.denote ctx = xPoly.denote' ctx → xPoly.denote' ctx = xPoly'.denote' ctx → p.denote' ctx = 0 := by
+  simp [eq_def_cert]; intro _ h₁ h₂; subst p; simp [h₁, h₂]
+  rw [← Int.sub_eq_add_neg, Int.sub_self]
+
 @[expose]
 def eq_def'_cert (x : Var) (e : Expr) (p : Poly) : Bool :=
   p == .add (-1) x e.norm
@@ -1922,6 +1927,15 @@ def eq_def'_cert (x : Var) (e : Expr) (p : Poly) : Bool :=
 theorem eq_def' (ctx : Context) (x : Var) (e : Expr) (p : Poly)
     : eq_def'_cert x e p → x.denote ctx = e.denote ctx → p.denote' ctx = 0 := by
   simp [eq_def'_cert]; intro _ h; subst p; simp [h]
+  rw [← Int.sub_eq_add_neg, Int.sub_self]
+
+@[expose]
+def eq_def'_norm_cert (x : Var) (e : Expr) (ePoly ePoly' p : Poly) : Bool :=
+  ePoly == e.norm && p == .add (-1) x ePoly'
+
+theorem eq_def'_norm (ctx : Context) (x : Var) (e : Expr) (ePoly ePoly' : Poly) (p : Poly)
+    : eq_def'_norm_cert x e ePoly ePoly' p → x.denote ctx = e.denote ctx → ePoly.denote' ctx = ePoly'.denote' ctx → p.denote' ctx = 0 := by
+  simp [eq_def'_norm_cert]; intro _ _ h₁ h₂; subst ePoly p; simp [h₁, ← h₂]
   rw [← Int.sub_eq_add_neg, Int.sub_self]
 
 theorem eq_norm_poly (ctx : Context) (p p' : Poly) : p.denote' ctx = p'.denote' ctx → p.denote' ctx = 0 → p'.denote' ctx = 0 := by
